working ppi interpreter

src/execute.ml
@@ -74,27 +74,34 @@ let tuple_drop_hs res =
   | (((_, s), f), r) -> ((s, f), r)
 
 let take_step verbosity _i cfg =
-  let ((s, _), _)  = (*Convert.from_triple*) cfg in
-  let res = run_step_compat cfg in
+  let res = run_step cfg in
+  (*
   let ((s', _), _)  = (*Convert.from_triple*) res in
   let store_status = if s = s' then "unchanged" else "changed" in
   debug_info result verbosity (fun _ ->
-    Printf.sprintf "%sand store %s\n%!" (pp_res_tuple_except_store (tuple_drop_hs res)) store_status) ;
+    Printf.sprintf "%sand store %s\n%!" (pp_res_tuple_except_store (tuple_drop_hs res)) store_status) ;*)
   match (*Convert.from_triple*) res with
-  | ((_, _), Extract.RS_crash _) ->
-    debug_info result verbosity ~style:red (fun _ -> "crash:") ;
+  | Extract.RSP_exhaustion ->
+    debug_info result verbosity ~style:red (fun _ -> "exhaustion:") ;
     debug_info result verbosity (fun _ -> " " ^ string_of_crash_reason ()) ;
     pure cfg
-  | ((_, _), Extract.RS_break _) ->
-    debug_info result verbosity ~style:red (fun _ -> "break") ;
+  | Extract.RSP_terminal _ ->
+    debug_info result verbosity ~style:red (fun _ -> "terminal") ;
     pure cfg
-  | ((_, _), Extract.RS_return vs) ->
-    debug_info result verbosity ~style:green (fun _ -> "return:") ;
-    debug_info result verbosity (fun _ -> " " ^ pp_values vs) ;
+  | Extract.RSP_cfg _ ->
     pure cfg
-  | ((s', vs'), Extract.RS_normal es) ->
-    pure ((s', vs'), es)
 
+
+
+let sies_to_cfg (name: string) sies = 
+  match lookup_exported_function name sies with
+  | None -> Error ("unknown function `" ^ name ^ "`")
+  | Some (((_, s), f), addr) -> 
+    match run_init_invoke s f addr with 
+    | Some cfg -> OK cfg
+    | None -> Error ("Invocation failed to typecheck")
+
+    (*
 let repl verbosity sies (name : string) =
   LNoise.set_hints_callback (fun line ->
       (* FIXME: Documentation is needed here. I don’t know what these lines do. *)
@@ -117,193 +124,96 @@ let repl verbosity sies (name : string) =
    "get tab completion with <TAB>";
    "type quit to exit gracefully"]
   |> List.iter print_endline;
-  let (((_, s), i), _) = sies in
-  match lookup_exported_function name sies with
-  | None -> error ("unknown function `" ^ name ^ "`")
-  | Some cfg0 ->
+  match sies_to_cfg name sies with
+  | Error err -> error err
+  | OK cfg0 ->
     debug_info result verbosity (fun _ ->
-      Printf.sprintf "\n%sand store\n%s\n%!"
-        (pp_config_tuple_except_store (tuple_drop_hs cfg0))
-        (pp_store 1 s)) ;
+      Printf.sprintf "\n%s"
+        (pp_res_tuple_except_store cfg0)) ;
     (fun from_user cfg ->
       if from_user = "quit" then exit 0;
       LNoise.history_add from_user |> ignore;
       LNoise.history_save ~filename:"history.txt" |> ignore;
-      if from_user = "" || from_user = "step" then take_step verbosity i cfg
-      else if from_user = "s" || from_user = "store" then
-        (let (((_, s), _), _) = cfg in
-         Printf.sprintf "%s%!" (pp_store 0 s) |> print_endline;
-         pure cfg)
+      if from_user = "" || from_user = "step" then take_step verbosity cfg
       else if from_user = "help" then
         (Printf.sprintf "commands:\nstep: take a step\nstore: display the store\nquit: quit\nhelp: this help message" |> print_endline;
          pure cfg)
       else (Printf.sprintf "unknown command" |> print_endline; pure cfg))
     |> (fun cb -> user_input "> " cb cfg0)
-
+*)
 let interpret verbosity error_code_on_crash sies (name: string) =
   let print_step_header gen =
     debug_info verbosity intermediate ~style:bold
       (fun () -> Printf.sprintf "step %d:\n" gen) in
- (* let print_exhaustion gen = 
+  (*let print_exhaustion gen = 
     debug_info verbosity intermediate ~style:bold
       (fun () -> Printf.sprintf "step %d: \n Execution halted due to fuel exhaustion\n" gen) in*)
   let* cfg0 =
     TopHost.from_out (
       ovpending verbosity stage "interpreting" (fun _ ->
-        match lookup_exported_function name sies with
-        | None -> Error ("unknown function `" ^ name ^ "`")
-        | Some cfg0 -> OK cfg0)) in
+        sies_to_cfg name sies
+        )) in
   let rec eval_cfg gen cfg =
    (* if (gen >= max_steps) then 
       (print_exhaustion gen;
       debug_info verbosity result ~style:bold (fun _ -> "fuel exhaustion\n");
       pure None)
     else *)
-      (let cfg_res = run_step_compat cfg in
+      (let cfg_res = run_step cfg in
       print_step_header gen ;
       debug_info verbosity intermediate
-        (fun _ -> pp_res_tuple_except_store (tuple_drop_hs cfg_res));
+        (fun _ -> pp_res_tuple_except_store_typed cfg_res);
+        (*
       debug_info_span verbosity intermediate intermediate
         (fun () ->
           let (((_, s), _), _) = cfg in
           let (((_, s'), _), _) = cfg_res in
           let store_status = if s = s' then "unchanged" else "changed" in
-          Printf.sprintf "and store %s\n" store_status);
+          Printf.sprintf "and store %s\n" store_status); 
       debug_info verbosity store
         (fun () ->
           let (((_, s'), _), _) = cfg_res in
-          Printf.sprintf "and store\n%s" (pp_store 1 s'));
+          Printf.sprintf "and store\n%s" (pp_store 1 s'));*)
       match cfg_res with
-      | (_, RS_crash _) ->
+      | Extract.RSP_exhaustion ->
         wait_message verbosity;
         debug_info verbosity result ~style:red (fun _ -> "crash\n");
         pure None
-      | (_, RS_break _) ->
+      | Extract.RSP_cfg (_, s, f, es, ts, p) ->
         wait_message verbosity;
-        debug_info verbosity result ~style:bold (fun _ -> "break\n");
-        pure None
-      | (_, RS_return vs) ->
-        wait_message verbosity;
-        debug_info verbosity result ~style:green (fun _ -> "return");
-        debug_info verbosity result (fun _ -> Printf.sprintf " %s\n" (pp_values vs));
-        pure (Some vs)
-      | (((hs', s'), vs'), RS_normal es) ->
+        debug_info verbosity result ~style:green (fun _ -> "cfg\n");
+        eval_cfg (gen + 1) cfg_res
+      | Extract.RSP_terminal (es, p) ->
         begin match is_const_list es with
         | Some vs -> 
           debug_info verbosity stage ~style:green (fun _ -> "success after " ^ string_of_int gen ^ " steps\n");
           pure (Some vs)
-        | None -> eval_cfg (gen + 1) ((((hs', s'), vs'), es))
+        | None -> 
+          debug_info verbosity stage ~style:red (fun _ -> "termination with a non-value\n"); 
+          pure None
         end) in
-
-  debug_info verbosity result ~style:yellow (fun _ -> "Context optimisation disabled\n");
+  
+  let start_time = Sys.time() in
+  debug_info verbosity result ~style:yellow (fun _ -> "PPI Interpreter\n");
   print_step_header 0 ;
   debug_info verbosity intermediate (fun _ ->
-    Printf.sprintf "\n%s\n" (pp_config_tuple_except_store (tuple_drop_hs cfg0)));
+    Printf.sprintf "\n%s\n" (pp_res_tuple_except_store_typed cfg0));
   let* res = eval_cfg 1 cfg0 in
   debug_info_span verbosity result stage (fun _ ->
     match res with
     | Some vs -> pp_values vs
     | None -> "");
+  Printf.printf "Execution time: %fs\n" (Sys.time() -. start_time);
   if error_code_on_crash && (match res with None -> true | Some _ -> false) then exit 1
   else pure ()
 
-  (*
-module Interpreter_ctx_extract :
- sig
-  val host_application_impl :
-    Equality.sort -> EmptyHost.store_record -> function_type -> Equality.sort
-    -> value list -> Equality.sort * (EmptyHost.store_record * result) option
-
-  val run_one_step_ctx : Equality.sort -> cfg_tuple_ctx -> run_step_ctx_result
-
-  val run_step_cfg_ctx_reform : cfg_tuple_ctx -> cfg_tuple_ctx option
-
-  val run_v_init :
-    Equality.sort store_record -> administrative_instruction list ->
-    cfg_tuple_ctx option
-
-  val es_of_cfg : cfg_tuple_ctx -> administrative_instruction list
- end
- *)
-
-include Extract.Interpreter_ctx_extract
-
-  let interpret_ctx verbosity error_code_on_crash sies (name: string) =
-    let print_step_header gen =
-      debug_info verbosity intermediate ~style:bold
-        (fun () -> Printf.sprintf "step %d:\n" gen) in
-   (* let print_exhaustion gen = 
-      debug_info verbosity intermediate ~style:bold
-        (fun () -> Printf.sprintf "step %d: \n Execution halted due to fuel exhaustion\n" gen) in*)
-    let* cfg0 =
-      TopHost.from_out (
-        ovpending verbosity stage "interpreting" (fun _ ->
-          match lookup_exported_function name sies with
-          | None -> Error ("unknown function `" ^ name ^ "`")
-          | Some cfg0 -> OK cfg0)) in
-    let rec eval_cfg gen (hs: Extract.Equality.sort) (cfg: Extract.cfg_tuple_ctx) =
-      (let run_step_res = run_one_step_ctx hs cfg in
-        print_step_header gen ;
-        match run_step_res with
-        | Extract.RSC_error ->
-          wait_message verbosity;
-          debug_info verbosity result ~style:red (fun _ -> "crash_error\n");
-          pure None
-        | Extract.RSC_invalid ->
-          wait_message verbosity;
-          debug_info verbosity result ~style:red (fun _ -> "crash_invalid\n");
-          pure None
-        | Extract.RSC_value vs ->
-          debug_info verbosity stage ~style:green (fun _ -> "success after " ^ string_of_int gen ^ " steps\n");
-          pure (Some vs)
-        | Extract.RSC_normal (hs_res, cfg_res) ->
-          debug_info verbosity intermediate
-          (fun () -> pp_es (es_of_cfg cfg_res)); 
-          debug_info verbosity intermediate
-          (fun () -> 
-            let (((s, _), _), _) = cfg in
-            let (((s', _), _), _) = cfg_res in 
-            let store_status = if s = s' then "unchanged" else "changed" in
-              Printf.sprintf "and store %s\n" store_status
-            ); 
-          debug_info verbosity store
-          (fun () ->
-            let (((s', _), _), _) = cfg_res in
-              Printf.sprintf "and store\n%s" (pp_store 1 s'));
-          (match run_step_cfg_ctx_reform cfg_res with
-          | Some cfg_res' -> eval_cfg (gen + 1) hs_res cfg_res'
-          | None -> pure None
-          )
-        ) in
-    print_step_header 0 ;
-
-    let (((hs, s), _), es) = cfg0 in
-    debug_info verbosity intermediate
-    (fun () -> pp_es es); 
-
-    let cfg_init = run_v_init s es in
-    (match cfg_init with
-    | Some cfg_init' ->
-      let* res = eval_cfg 0 hs cfg_init' in
-      (debug_info_span verbosity result stage (fun _ ->
-        match res with
-        | Some vs -> pp_values vs
-        | None -> ""
-        );
-        if error_code_on_crash && (match res with None -> true | Some _ -> false) then exit 1
-        else pure ()
-      )
-    | None -> debug_info verbosity result ~style:red (fun _ -> "invalid starting es\n"); exit 1
-    )
-
 (* TODO: update the interactive to use the context-optimised version as well *)
-let instantiate_interpret verbosity interactive no_ctx_optimise error_code_on_crash m name =
+let instantiate_interpret verbosity interactive error_code_on_crash m name =
   let* store_inst_exps =
     TopHost.from_out (
       ovpending verbosity stage "instantiation" (fun _ ->
         match interp_instantiate_wrapper m with
         | None -> Error "instantiation error"
         | Some (store_inst_exps, _) -> OK store_inst_exps)) in
-  if interactive then repl verbosity store_inst_exps name
-  else if no_ctx_optimise then interpret verbosity error_code_on_crash store_inst_exps name
-  else interpret_ctx verbosity error_code_on_crash store_inst_exps name
+  if interactive then (*repl*) interpret verbosity error_code_on_crash store_inst_exps name
+  else interpret verbosity error_code_on_crash store_inst_exps name
